\begin{eqnarray}
	\bm{Y_L}&=&\left[
	\begin{array}{c}
	\dfrac{L_{(1)}}{\dfrac{1}{2} \rho S V_{a(1)}^2} - C_{L_0} - C_{L_\alpha}\alpha_{(1)}
	\\ \vdots \\
    \dfrac{L_{(n)}}{\dfrac{1}{2} \rho S V_{a(n)}^2} - C_{L_0} - C_{L_\alpha}\alpha_{(n)}
	\end{array}
	\right]

  \bm{X_L}&=&\left[
  	\begin{array}{ccc}
  	\dfrac{c}{2 V_{a(1)}} \dot{\Theta}_{(1)}  & \delta_{e(1)}  & \dfrac{1}{\dfrac{1}{2} \rho V_{a(1)} S}  \\
  	\vdots & \vdots & \vdots \\
  	\dfrac{c}{2 V_{a(n)}} \dot{\Theta}_{(n)}  & \delta_{e(n)}  & \dfrac{1}{\dfrac{1}{2} \rho V_{a(n)} S}  \\
  	\end{array}
  	\right]

\begin{align}
	\dot{u} &= -qw - g\sin\Theta + \dfrac{T_m}{m}\sin\gamma + \dfrac{X}{m} \\
	\dot{w} &= -qu + g\cos\Theta - \dfrac{T_m\cos\gamma - (T_r+T_f)}{m} - \dfrac{Z}{m} \\
	\dot{q} &= \dfrac{M}{I_{yy}} \\
	\dot{\theta} &= q
	\end{align}
